multi-steps

plf/Smallstep.v
@@ -17,3 +17,145 @@ Fixpoint evalF (t : tm) : nat :=
   | C n => n
   | P t1 t2 => evalF t1 + evalF t2
   end.
+
+Inductive step : tm -> tm -> Prop :=
+| ST_PlusConstConst : forall n1 n2,
+    (step
+       (P (C n1) (C n2))
+       (C (n1 + n2)))
+| ST_Plus1 : forall t1 t1' t2,
+    (step t1 t1') -> (step (P t1 t2)
+                          (P t1' t2))
+| ST_Plus2 : forall n1 t2 t2',
+    (step t2 t2') -> (step (P (C n1) t2)
+                          (P (C n1) t2')).
+
+Notation " t '-->' t' " := (step t t') (at level 50, left associativity).
+Example test_step_1 :
+      P
+        (P (C 1) (C 3))
+        (P (C 2) (C 4))
+      -->
+      P
+        (C 4)
+        (P (C 2) (C 4)).
+Proof.
+  apply ST_Plus1.
+  apply ST_PlusConstConst.
+Qed.
+
+Example test_step_2 :
+      P
+        (C 0)
+        (P
+          (C 2)
+          (P (C 1) (C 3)))
+      -->
+      P
+        (C 0)
+        (P
+          (C 2)
+          (C 4)).
+Proof.
+  apply ST_Plus2.
+  apply ST_Plus2.
+  apply ST_PlusConstConst.
+Qed.
+
+
+Definition relation (X : Type) := X -> X -> Prop.
+
+Inductive value : tm -> Prop :=
+  | v_const : forall n, value (C n).
+
+Module Temp4.
+
+  Inductive tm1 : Type :=
+  | tru : tm1
+  | fls : tm1
+  | test : tm1 -> tm1 -> tm1 -> tm1.
+
+  Inductive value : tm1 -> Prop :=
+  | v_tru : value tru
+  | v_fls : value fls.
+
+  Inductive step1 : tm1 -> tm1 -> Prop :=
+  | ST_IfTrue : forall t1 t2,
+      (step1 (test tru t1 t2)
+             t1)
+  | ST_IfFalse : forall t1 t2,
+      (step1 (test fls t1 t2)
+             t2)
+  | ST_If : forall t1 t1' t2 t3,
+      (step1 t1 t1') ->
+      (step1 (test t1 t2 t3)
+            (test t1' t2 t3)).
+  Notation " t '--->' t' " := (step1 t t') (at level 40).
+
+  Definition bool_step_propl :=
+    fls ---> fls.
+
+End Temp4.
+
+(* Multi-Step Reduction *)
+Inductive multi {X : Type} (R : relation X) : relation X :=
+| multi_refl : forall (x : X), multi R x x
+| multi_step : forall (x y z : X), R x y -> multi R y z -> multi R x z.
+
+Notation " t '-->*' t' " := (multi step t t') (at level 40).
+
+Theorem multi_R : forall (X : Type) (R : relation X) (x y : X),
+    R x y -> (multi R) x y.
+Proof.
+  intros.
+  apply multi_step with y.
+  apply H.
+  apply multi_refl.
+Qed.
+
+Theorem multi_trans :
+  forall (X : Type) (R : relation X) (x y z : X),
+    multi R x y -> multi R y z -> multi R x z.
+Proof.
+  intros.
+  induction H.
+  - assumption.
+  - apply multi_step with y.
+    assumption.
+    apply IHmulti.
+    apply H0.
+Qed.
+
+Lemma test_multistep_1:
+      P
+        (P (C 0) (C 3))
+        (P (C 2) (C 4))
+   -->*
+      C ((0 + 3) + (2 + 4)).
+Proof.
+  apply multi_step with
+      (P (C (0 + 3))
+         (P (C 2) (C 4))).
+  apply ST_Plus1.
+  apply ST_PlusConstConst.
+  apply multi_step with
+      (P (C (0 + 3))
+         (C (2 + 4))).
+  apply ST_Plus2.
+  apply ST_PlusConstConst.
+  apply multi_R.
+  apply ST_PlusConstConst.
+Qed.
+
+Inductive ev : nat -> Prop :=
+| ev_0 : ev 0
+| ev_SS : forall n, ev n -> ev (S (S n)).
+
+Check ev_SS.
+
+Check ev_SS 4 (ev_SS 2 (ev_SS 0 ev_0)).
+
+
+
+
+
